Capless/Weakening/Subtyping.lean
@@ -1,0 +1,59 @@
+import Capless.Renaming.Term.Subtyping
+import Capless.Renaming.Type.Subtyping
+import Capless.Renaming.Capture.Subtyping
+namespace Capless
+
+theorem SSubtyp.weaken
+  (h : SSubtyp Γ S1 S2) :
+  ∀ b, SSubtyp (Γ.var b) S1.weaken S2.weaken := by
+  intro b
+  simp [SType.weaken]
+  apply SSubtyp.rename
+  { apply h }
+  { apply VarMap.weaken }
+
+theorem CSubtyp.weaken
+  (h : CSubtyp Γ E1 E2) :
+  CSubtyp (Γ.var T) E1.weaken E2.weaken := by
+  simp [CType.weaken]
+  apply CSubtyp.rename
+  { apply h }
+  { apply VarMap.weaken }
+
+theorem ESubtyp.weaken
+  (h : ESubtyp Γ E1 E2) :
+  ESubtyp (Γ.var T) E1.weaken E2.weaken := by
+  simp [EType.weaken]
+  apply ESubtyp.rename
+  { apply h }
+  { apply VarMap.weaken }
+
+theorem SSubtyp.tweaken
+  (h : SSubtyp Γ S1 S2) :
+  SSubtyp (Γ.tvar b) S1.tweaken S2.tweaken := by
+  simp [SType.tweaken]
+  apply? SSubtyp.trename
+  apply TVarMap.weaken
+
+theorem ESubtyp.tweaken
+  (h : ESubtyp Γ E1 E2) :
+  ESubtyp (Γ.tvar b) E1.tweaken E2.tweaken := by
+  simp [EType.tweaken]
+  apply? ESubtyp.trename
+  apply TVarMap.weaken
+
+theorem ESubtyp.cweaken
+  (h : ESubtyp Γ E1 E2) :
+  ESubtyp (Γ.cvar b) E1.cweaken E2.cweaken := by
+  apply? ESubtyp.crename
+  apply CVarMap.weaken
+
+theorem SSubtyp.cweaken
+  (h : SSubtyp Γ S1 S2) :
+  ∀ b, SSubtyp (Γ.cvar b) S1.cweaken S2.cweaken := by
+  intro b
+  simp [SType.cweaken]
+  apply? SSubtyp.crename
+  apply CVarMap.weaken
+
+end Capless
