Capless/Weakening/Typing.lean
@@ -1,0 +1,28 @@
+import Capless.Renaming.Term.Typing
+import Capless.Renaming.Type.Typing
+import Capless.Renaming.Capture.Typing
+namespace Capless
+
+theorem Typed.weaken
+  (h : Typed Γ t E) :
+  Typed (Γ.var T) t.weaken E.weaken := by
+  simp [Term.weaken, EType.weaken]
+  apply Typed.rename h
+  apply VarMap.weaken
+
+def Typed.tweaken
+  (h : Typed Γ t E) :
+  Typed (Γ.tvar b) t.tweaken E.tweaken := by
+  simp [Term.tweaken, EType.tweaken]
+  apply h.trename
+  apply TVarMap.weaken
+
+def Typed.cweaken
+  (h : Typed Γ t E) :
+  Typed (Γ.cvar b) t.cweaken E.cweaken := by
+  simp [Term.cweaken, EType.cweaken]
+  apply h.crename
+  apply CVarMap.weaken
+
+
+end Capless
