Capless/playground.lean
@@ -1,0 +1,15 @@
+inductive MemKind: Type -- classifies names/members
+| field -- names of term members
+| type  -- names of type members
+
+inductive Ty: Nat -> Type -- for simplicity, just one case
+| bot: Ty n
+
+inductive ComponentSig: Nat -> MemKind -> Type -- classifies the dependent second component of a pair _type_
+| field : Ty n -> ComponentSig n field         -- field member of type T
+| type  : Ty n -> Ty n -> ComponentSig n type  -- type member with interval S .. T
+
+def ComponentSig.interval' (sig : ComponentSig n K) : Ty n × Ty n := by
+  cases sig
+  case field => sorry
+  case type => sorry
